refactor: add manual proof and add modifies function

ISLPrograms.fst
@@ -2,6 +2,8 @@ module ISLPrograms
 
 open IncSepLogic
 
+open FStar.Classical
+
 (*
 n := 1000000;
 i, j := 0;
@@ -20,14 +22,14 @@ let ge (x y : expr) : expr = enot (Lt x y)
 // n := 1000000; i := 0; j := 0;
 unfold let init_vars = 
   Assign "n" (Const 1000000) `Seq`
-  Assign "i" (Const 0) `Seq`
-  Assign "j" (Const 0)
+  (Assign "i" (Const 0) `Seq`
+  Assign "j" (Const 0))
 
 // el cuerpo del while
 let loop_body =
   Assume (Lt (Var "i") (Var "n")) `Seq`
-  Assign "i" (Plus (Var "i") (Const 1)) `Seq`
-  (Assign "j" (Plus (Var "j") (Const 1)) ||| Skip)
+  (Assign "i" (Plus (Var "i") (Const 1)) `Seq`
+  (Assign "j" (Plus (Var "j") (Const 1)) ||| Skip))
 
 let assert_stmt =
   Seq (Assume (Eq (Var "j") (Var "n"))) Error |||
@@ -39,6 +41,121 @@ unfold let prog1 =
   Assume (ge (Var "i") (Var "n")) `Seq`
   assert_stmt
 
+let cond_false : cond =
+  fun _ -> false
+
+// estado inicial
+let pre_vacia : cond =
+  fun _ -> true
+
+let post_er_bug : cond =
+  fun (st, hp) -> st "n" == Nat 1000000 /\ st "i" == Nat 1000000 /\ st "j" == Nat 1000000
+
+unfold let state_k (k : nat) : cond =
+  fun (st, hp) -> st "n" == Nat 1000000 /\ st "i" == Nat k /\ st "j" == Nat k
+
+unfold let mid_i (k : nat) : cond =
+  fun (st, hp) -> st "n" == Nat 1000000 /\ st "i" == Nat (k + 1) /\ st "j" == Nat k
+
+// prueba init_vars
+let test_init () : GTot (isl_triple pre_vacia init_vars (state_k 0) cond_false) =
+  let p_n = ISL_Assign #pre_vacia "n" (Const 1000000) in
+  let p_i = ISL_Assign #_ "i" (Const 0) in
+  let p_j = ISL_Assign #_ "j" (Const 0) in
+
+  let p_ij = ISL_Seq p_i p_j in
+  let p_init = ISL_Seq p_n p_ij in
+
+  ISL_Consequence pre_vacia (state_k 0) cond_false p_init () () ()
+
+let lemma_inc_i (k : nat) (x : state)
+  : Lemma (requires (mid_i k x))
+          (ensures (let st, hp = x in
+                    exists (x_init : store). state_k k (x_init, hp) /\
+                    st "i" == Nat (eval_expr (x_init, hp) (Plus (Var "i") (Const 1))) /\
+                    (forall y. y <> "i" ==> st y == x_init y))) =
+  let st, hp = x in
+  let x_init : store = fun y ->
+    if y = "i" then Nat k
+    else st y
+  in
+
+  exists_intro (fun x_init ->
+    state_k k (x_init, hp) /\
+    st "i" == Nat (eval_expr (x_init, hp) (Plus (Var "i") (Const 1))) /\
+    (forall y. y <> "i" ==> st y == x_init y)) x_init
+
+let lemma_inc_j (k : nat) (x : state)
+  : Lemma (requires (state_k (k + 1) x))
+          (ensures (let st, hp = x in
+                    exists x_init. mid_i k (x_init, hp) /\
+                    st "j" == Nat (eval_expr (x_init, hp) (Plus (Var "j") (Const 1))) /\
+                    (forall y. y <> "j" ==> st y == x_init y))) =
+  let st, hp = x in
+  let x_init : store = fun y ->
+    if y = "j" then Nat k
+    else st y
+  in
+
+  exists_intro (fun x_init ->
+    mid_i k (x_init, hp) /\
+    st "j" == Nat (eval_expr (x_init, hp) (Plus (Var "j") (Const 1))) /\
+    (forall y. y <> "j" ==> st y == x_init y)) x_init
+
+let test_1step (k : nat{k < 1000000}) : GTot (isl_triple (state_k k) loop_body (state_k (k + 1)) cond_false) =
+  let p_assume_raw = ISL_Assume #(state_k k) (Lt (Var "i") (Var "n")) in
+  let p_assume = ISL_Consequence (state_k k) (state_k k) cond_false p_assume_raw () () () in
+
+  let p_i_raw = ISL_Assign #(state_k k) "i" (Plus (Var "i") (Const 1)) in
+  let _ = forall_intro (move_requires (lemma_inc_i k)) in
+  let p_i = ISL_Consequence (state_k k) (mid_i k) cond_false p_i_raw () () () in
+
+  let p_j_raw = ISL_Assign #(mid_i k) "j" (Plus (Var "j") (Const 1)) in
+  let _ = forall_intro (move_requires (lemma_inc_j k)) in
+  let p_j_branch = ISL_Consequence (mid_i k) (state_k (k + 1)) cond_false p_j_raw () () () in
+  let p_j = ISL_ChoiceL p_j_branch in
+
+  let p_ij = ISL_Seq p_i p_j in
+  let p_raw = ISL_Seq p_assume p_ij in
+  ISL_Consequence (state_k k) (state_k (k + 1)) cond_false p_raw () () ()
+
+let rec test_loop (k : nat{k <= 1000000}) : GTot (isl_triple (state_k 0) (Kleene loop_body) (state_k k) cond_false) =
+  if k = 0 then
+    let p_base = ISL_Kleene0 #loop_body #(state_k 0) in
+    ISL_Consequence (state_k 0) (state_k k) cond_false p_base () () ()
+  
+  else
+    let p_prev = test_loop (k - 1) in
+    let p_step = test_1step (k - 1) in
+
+    let p_seq_raw = ISL_Seq p_prev p_step in
+    let p_seq = ISL_Consequence (state_k 0) (state_k k) cond_false p_seq_raw () () () in
+    ISL_KleeneS p_seq
+
+let test_assert () : GTot (isl_triple (state_k 1000000) (Seq (Assume (Eq (Var "i") (Var "n"))) assert_stmt) cond_false post_er_bug) =
+  let p_exit_raw = ISL_Assume #(state_k 1000000) (Eq (Var "i") (Var "n")) in
+  let p_exit = ISL_Consequence (state_k 1000000) (state_k 1000000) cond_false p_exit_raw () () () in
+
+  let p_cond_err = ISL_Assume #(state_k 1000000) (Eq (Var "j") (Var "n")) in
+  let p_err = ISL_Error #_ in
+  let p_branch_err = ISL_Seq p_cond_err p_err in
+
+  let p_assert = ISL_ChoiceL p_branch_err in
+  let p_raw = ISL_Seq p_exit p_assert in
+  ISL_Consequence (state_k 1000000) cond_false post_er_bug p_raw () () ()
+
+let test1 () : GTot (isl_triple pre_vacia
+  (Seq init_vars
+       (Seq (Kleene loop_body)
+            (Seq (Assume (Eq (Var "i") (Var "n"))) assert_stmt)))
+                 cond_false
+                 post_er_bug) =
+  let triple_seq =
+    ISL_Seq (test_init ())
+            (ISL_Seq (test_loop 1000000)
+                     (test_assert ()))
+  in
+  ISL_Consequence pre_vacia cond_false post_er_bug triple_seq () () ()
 
 (*
   {true}
